compcertox/Composition.v
@@ -202,30 +202,104 @@ Section HCOMP.
 End HCOMP.
 
 Require Import TensorComp.
+(* Overriding notations *)
+Import Smallstep_.
+
+(* Any call into the empty layer yields undefined behavior *)
+
+Definition empty_ident := 1%positive.
+
+Definition empty_layer {K}: semantics li_null (li_c@K):=
+  {|
+    skel := AST.mkprogram nil nil empty_ident;
+    state := Empty_set;
+    footprint id := False;
+    activate se :=
+      {|
+        genvtype := unit;
+        globalenv := tt;
+        step _ _ _ _ := False;
+        initial_state _ _ := False;
+        at_external _ _ := False;
+        after_external _ _ _ := False;
+        final_state _ _ := False;
+      |};
+  |}.
+
+Lemma empty_sk_bot {K}: forall sk, linkorder (skel (@empty_layer K)) sk.
+Admitted.
+
+Generalizable All Variables.
+
+Section APPROX.
+  Context {E1 E2: Type}.
+  Context (LM LN: semantics li_c li_c).
+  Let LMN i := match i with true => LM | false => LN end.
+  Context `(M: mem_ops).
+  Variable (sk: AST.program unit unit).
+
+  Let L1 := comp_semantics' (LM @ E1) empty_layer sk.
+  Let L2 := comp_semantics' (LN @ E2) empty_layer sk.
+  Let L := comp_semantics' ((SmallstepLinking_.semantics' LMN sk) @ (E1 * E2)) empty_layer sk.
+
+  Lemma tensor_composition_approximation:
+    Layer.tensor_semantics' L1 L2 M sk ≤ L.
+  Admitted.
+
+End APPROX.
+
+Notation "R1 ⊗ R2" := (tcomp_rel R1 R2) (left associativity, at level 50): krel_scope.
 
 Section TCOMP.
 
-  Generalizable All Variables.
   Context {M N: cmodule}
-          `{R: rel_adt Kr1 Kr2} `{S: rel_adt Ks1 Ks2}
-          `(HL1: ksim L1 L3 M R) `(HL2: ksim L2 L4 N S).
+          (* The C implement is supposed to be closed programs so E1 and E2 will
+             be abstract data of the unit type or a product of the unit type if
+             the implementation is a composition of several primitive layers *)
+          `{R: rel_adt K1 E1} `{S: rel_adt K2 E2}
+          `(HL1: ksim L1 empty_layer M R) `(HL2: ksim L2 empty_layer N S).
   Variable (sk: AST.program unit unit).
-  Hypothesis (Hk1: linkorder (skel L1) sk) (Hk2: linkorder (skel L2) sk)
-             (Hk3: linkorder (skel L3) sk) (Hk4: linkorder (skel L4) sk).
+  Hypothesis (Hk1: linkorder (skel L1) sk) (Hk2: linkorder (skel L2) sk).
+  Context (INV: CallConv_Invariants R S).
 
-  Let K1 := fun (i : bool) => if i then Kr1 else Ks1.
-  Let K2 := fun (i : bool) => if i then Kr2 else Ks2.
-
-  Let La := Tensor.tensor_semantics' K1 (fun (i: bool) => match i with true => L1 | false => L2 end) sk.
-  Let Lb := Tensor.tensor_semantics' K2 (fun (i: bool) => match i with true => L3 | false => L4 end) sk.
-
-  Definition RS: rel_adt (forall i, K1 i) (forall i, K2 i).
-  Proof.
-    apply tcomp_rel. intros [|]; eauto.
-  Qed.
+  (* The memory operations used in the layer composition is irrelevant because
+     the layer interface only updates the abstract data. So theoretically we
+     can feed whatever mem_ops to the definition and it should be provable *)
+  Let L := Layer.tensor_semantics' L1 L2 INV sk.
 
   Lemma layer_tcomp:
-    ksim La Lb (M ++ N) RS.
+    ksim L empty_layer (M ++ N) (R ⊗ S).
+  Proof.
+    unfold ksim in *.
+    destruct HL1 as [Hsk1 [Hmod1 H1]]. clear HL1.
+    destruct HL2 as [Hsk2 [Hmod2 H2]]. clear HL2.
+    split. eapply linkorder_trans; eauto.
+    split. apply compatible_app; (eapply compatible_trans; [ | eauto]); eauto.
+    clear Hsk1 Hmod1 Hsk2 Hmod2.
+
+    eapply open_fsim_ccref. apply cc_compose_id_left.
+    unfold flip. apply cc_compose_id_right.
+    eapply compose_forward_simulations.
+    {
+      eapply Layer.tensor_compose_simulation'; eauto.
+    }
+
+    etransitivity.
+    {
+      replace (skel L1) with sk.
+      replace (skel L2) with sk.
+      apply tensor_composition_approximation.
+      admit.
+      admit.
+    }
+
+    unfold layer_comp.
+
+    eapply categorical_compose_simulation'.
+    - apply lifting_simulation. eapply cmodule_app_simulation.
+    - reflexivity.
+    - apply linkorder_refl.
+    - apply empty_sk_bot.
   Admitted.
 
 End TCOMP.
