compcertox/TensorComp.v
@@ -5,119 +5,205 @@ Require Import CallconvAlgebra_.
 Require Import LanguageInterface_ Events Globalenvs Smallstep_ CategoricalComp FlatComp.
 Require Import Memory Values.
 Require Import Linking.
-Require Import Lifting.
+Require Import Lifting AbstractStateRel.
 
-Section COMP.
-  (* TODO: notation precedence *)
-  Context {I} (K: I -> Type)
-          {liA liB} (L: forall i, semantics (liA@(K i)) (liB@(K i))).
+Generalizable All Variables.
 
-  Notation Ki := (forall i, K i).
+Class mem_ops: Type :=
+  {
+    split: mem -> mem * mem;
+    combine: mem * mem -> mem;
+  }.
 
-  Hypothesis I_dec: forall (i j: I), {i = j} + {i <> j}.
+Class CallConv_Invariants `(cca: callconv (li_c@K1a) (li_c@K2a))
+      `(ccb: callconv (li_c@K1b) (li_c@K2b)) :=
+  {
+    op :> mem_ops;
 
-  Definition update_at (k: Ki) (j: I) (kj: K j): Ki.
-  Proof.
-    intros i. destruct (I_dec i j).
-    - subst. exact kj.
-    - exact (k i).
-  Defined.
+    (* For certified abstraction layers, the calling conventions essentially
+       captures the abstraction from concrete C values in particular memory
+       blocks to abstract data. The other memory blocks in the memory should not
+       affect the abstraction relation. For example, in the following diagram,
+       `m2a` is part of a larger memory `m2` and the abstract relation from the
+       calling convention `cca` translates `m2a` to abstract data in
+       `k1a`. Then, if we extract the same blocks from the source program memory
+       `m1` and obtain `m1a`, we get the "core" of the abstraction
+       relation. That is to say, if we have (m1, k1a) related to (m2, k2a), we
+       can strip off the unused blocks from `m1` and `m2` to get the fact that
+       (m1a, k1a) is related to (m2a, k1a). For the other hand, if we have (m1a,
+       k1a) related to (m2a, k2a), we can add a few extra blocks into the memory
+       as long as they don't interfere the blocks in the "core" part
 
-  Section WITH_SE.
-    Context (se: Genv.symtbl).
+       In the end, the operations in `mem_ops` are parametrized by the "core" of
+       the abstraction relations, which should be several block identifiers. The
+       layers being composed in this ways should not interfering private states
+       so the composition on the abstraction relations should witness an
+       evidence of such non-interference, which I think can be interpreted as a
+       pair of split and combine operations. (Maybe a few more extra properties
+       are required) *)
 
-    Variant tensor_state :=
-      tensor_st (i: I) (s:  Smallstep_.state (L i)) (k: Ki).
+    (*
+       (m1a, _)  k1a             m1a   k1a
+         |      / |               |    /|
+         |     /  |      <-->     |   / |
+         |    /   |               |  /  |
+         |   /    |               | /   |
+       (m2a, _)  k2a             m2a   k2a  *)
 
-    Inductive tensor_step: tensor_state -> trace -> tensor_state -> Prop :=
-    | step_intro i s t s' k:
-        Step (L i se) s t s' ->
-        tensor_step (tensor_st i s k) t (tensor_st i s' k).
+    (* Extract the "core" part from an inclusive abstraction relation *)
+    match_query_core1 wa vf1 args1 sg1 m1 k1a vf2 args2 sg2 m2 k2a:
+      match_query cca wa ((cq vf1 args1 sg1 m1), k1a) ((cq vf2 args2 sg2 m2), k2a) ->
+      let '(m1a, _) := split m1 in
+      let '(m2a, _) := split m2 in
+      match_query cca wa ((cq vf1 args1 sg1 m1a), k1a) ((cq vf2 args2 sg2 m2a), k2a);
 
-    Inductive tensor_initial_state: query (liB@Ki) -> tensor_state -> Prop :=
-    | initial_state_intro i s k q:
-        initial_state (L i se) (q, k i) s ->
-        tensor_initial_state (q, k) (tensor_st i s k).
+    match_query_core2 wb vf1 args1 sg1 m1 k1b vf2 args2 sg2 m2 k2b:
+      match_query ccb wb ((cq vf1 args1 sg1 m1), k1b) ((cq vf2 args2 sg2 m2), k2b) ->
+      let '(_, m1b) := split m1 in
+      let '(_, m2b) := split m2 in
+      match_query ccb wb ((cq vf1 args1 sg1 m1b), k1b) ((cq vf2 args2 sg2 m2b), k2b);
 
-    Inductive tensor_at_external: tensor_state -> query (liA@Ki) -> Prop :=
-    | at_external_intro i s k q kq k':
-        (forall j, i <> j -> k j = k' j) -> k' i = kq ->
-        at_external (L i se) s (q, kq) ->
-        tensor_at_external (tensor_st i s k) (q, k').
+    (* Add several extras blocks to the "core" part of the abstraction relation *)
+    match_reply_core1 wa ret1 m1a k1a ret2 m2a k2a m1b m2b:
+      match_reply cca wa ((cr ret1 m1a), k1a) ((cr ret2 m2a), k2a) ->
+      let m1 := combine (m1a, m1b) in
+      let m2 := combine (m2a, m2b) in
+      match_reply cca wa ((cr ret1 m1), k1a) ((cr ret2 m2), k2a);
 
-    Inductive tensor_after_external:
-      tensor_state -> reply (liA@Ki) -> tensor_state -> Prop :=
-    | after_external_intro i s s' k k' r kr:
-        (forall j, i <> j -> k j = k' j) -> k' i = kr ->
-        after_external (L i se) s (r, kr) s' ->
-        tensor_after_external (tensor_st i s k) (r, k') (tensor_st i s' k').
+    match_reply_core2 wb ret1 m1a k1b ret2 m2a k2b m1b m2b:
+      match_reply ccb wb ((cr ret1 m1b), k1b) ((cr ret2 m2b), k2b) ->
+      let m1 := combine (m1a, m1b) in
+      let m2 := combine (m2a, m2b) in
+      match_reply ccb wb ((cr ret1 m1), k1b) ((cr ret2 m2), k2b);
 
-    Inductive tensor_final_state: tensor_state -> reply (liB@Ki) -> Prop :=
-    | final_state_intro i s k k' r kr:
-        (forall j, i <> j -> k j = k' j) -> k' i = kr ->
-        final_state (L i se) s (r, kr) ->
-        tensor_final_state (tensor_st i s k) (r, k').
+    (* The invariant is essentially a relation represents the following
+       diagram. We need it for matching the states of the inactive component. *)
+    (*
+        m1a     k1a
+         |     / |
+         |    /  |
+         |   /   |
+         |  /    |
+         | /     |
+        m2a     k2a
+     *)
+    inv1: ccworld cca -> mem * K1a -> mem * K2a -> Prop;
+    inv2: ccworld ccb -> mem * K1b -> mem * K2b -> Prop;
 
-  End WITH_SE.
+    inv1_pre q1 q2 k1a k2a wa:
+      match_query cca wa (q1, k1a) (q2, k2a) ->
+      let 'cq _ _ _ m1 := q1 in
+      let 'cq _ _ _ m2 := q2 in
+      let '(m1a, _) := split m1 in
+      let '(m2a, _) := split m2 in
+      inv1 wa (m1a, k1a) (m2a, k2a);
 
-  Program Definition tensor_semantics' sk: semantics (liA@Ki) (liB@Ki) :=
-    {|
-      activate se :=
-        {|
-          step ge := tensor_step se;
-          initial_state := tensor_initial_state se;
-          at_external := tensor_at_external se;
-          after_external := tensor_after_external se;
-          final_state := tensor_final_state se;
-          globalenv := tt;
-        |};
-      skel := sk;
-      footprint id := exists i, footprint (L i) id;
-    |}.
+    inv1_post wa wb ret1 ret2 m1a k1a m2a k2a m1b' m2b' k1b' k2b':
+      inv1 wa (m1a, k1a) (m2a, k2a) ->
+      let r1 := cr ret1 (combine (m1a, m1b')) in
+      let r2 := cr ret2 (combine (m2a, m2b')) in
+      match_reply ccb wb (cr ret1 m1b', k1b') (cr ret2 m2b', k2b') ->
+      match_reply cca wa (r1, k1a) (r2, k2a);
 
-End COMP.
+    inv2_pre q1 q2 k1b k2b wb:
+      match_query ccb wb (q1, k1b) (q2, k2b) ->
+      let 'cq _ _ _ m1 := q1 in
+      let 'cq _ _ _ m2 := q2 in
+      let '(_, m1b) := split m1 in
+      let '(_, m2b) := split m2 in
+      inv2 wb (m1b, k1b) (m2b, k2b);
 
-(* This module defines tensor produce specific to layers. This is the same as the general one defined above
-   where the outgoing language interface replaced by li_null. Later, we expect
-   to find a trick to let Coq identify li_null and li_null@K  *)
-Module Tensor.
-  (* TODO: notation precedence *)
+    inv2_post wa wb ret1 ret2 m1b k1b m2b k2b m1a' m2a' k1a' k2a':
+      inv2 wb (m1b, k1b) (m2b, k2b) ->
+      let r1 := cr ret1 (combine (m1a', m1b)) in
+      let r2 := cr ret2 (combine (m2a', m2b)) in
+      match_reply cca wa (cr ret1 m1a', k1a') (cr ret2 m2a', k2a') ->
+      match_reply ccb wb (r1, k1b) (r2, k2b);
+
+  }.
+
+Coercion op: CallConv_Invariants >-> mem_ops.
+
+Module Layer.
+
   Section COMP.
-    Context {I} (K: I -> Type)
-            {li} (L: forall i, semantics li_null (li@(K i))).
-
-    Notation Ki := (forall i, K i).
+    Context {K1 K2: Type}.
+    Context (L1: semantics li_null (li_c@K1)) (L2: semantics li_null (li_c@K2)).
+    Context (M: mem_ops).
 
     Section WITH_SE.
       Context (se: Genv.symtbl).
 
       Variant tensor_state :=
-        tensor_st (i: I) (s:  Smallstep_.state (L i)) (k: Ki).
+      | tensor_st1 (s:  Smallstep_.state L1) (m: mem) (k: K2)
+      | tensor_st2 (s:  Smallstep_.state L2) (m: mem) (k: K1).
 
       Inductive tensor_step: tensor_state -> trace -> tensor_state -> Prop :=
-      | step_intro i s t s' k:
-          Step (L i se) s t s' ->
-          tensor_step (tensor_st i s k) t (tensor_st i s' k).
+      | tensor_step1 s t s' m k:
+          Step (L1 se) s t s' ->
+          tensor_step (tensor_st1 s m k) t (tensor_st1 s' m k)
+      | tensor_step2 s t s' m k:
+          Step (L2 se) s t s' ->
+          tensor_step (tensor_st2 s m k) t (tensor_st2 s' m k).
 
-      Inductive tensor_initial_state: query (li@Ki) -> tensor_state -> Prop :=
-      | initial_state_intro i s k q:
-          initial_state (L i se) (q, k i) s ->
-          tensor_initial_state (q, k) (tensor_st i s k).
+      Inductive tensor_initial_state: query (li_c@(K1 * K2)) -> tensor_state -> Prop :=
+      | initial_state1 s k1 k2 vf sg args m:
+          let ms := split m in
+          initial_state (L1 se) (cq vf sg args (fst ms), k1) s ->
+          tensor_initial_state ((cq vf sg args m), (k1, k2)) (tensor_st1 s (snd ms) k2)
+      | initial_state2 s k1 k2 vf sg args m:
+          let ms := split m in
+          initial_state (L2 se) (cq vf sg args (snd ms), k2) s ->
+          tensor_initial_state ((cq vf sg args m), (k1, k2)) (tensor_st2 s (fst ms) k1).
 
       Inductive tensor_at_external: tensor_state -> query li_null -> Prop := .
 
       Inductive tensor_after_external:
         tensor_state -> reply li_null -> tensor_state -> Prop := .
 
-      Inductive tensor_final_state: tensor_state -> reply (li@Ki) -> Prop :=
-      | final_state_intro i s k k' r kr:
-          (forall j, i <> j -> k j = k' j) -> k' i = kr ->
-          final_state (L i se) s (r, kr) ->
-          tensor_final_state (tensor_st i s k) (r, k').
+      Inductive tensor_final_state: tensor_state -> reply (li_c@(K1 * K2)) -> Prop :=
+      | final_state1 s k1 k2 ret m1 m2:
+          let m := combine (m1, m2) in
+          final_state (L1 se) s ((cr ret m1), k1) ->
+          tensor_final_state (tensor_st1 s m2 k2) ((cr ret m), (k1, k2))
+      | final_state2 s k1 k2 ret m1 m2:
+          let m := combine (m1, m2) in
+          final_state (L2 se) s ((cr ret m2), k2) ->
+          tensor_final_state (tensor_st2 s m1 k1) ((cr ret m), (k1, k2)).
+
+      Lemma star_tensor_step1 s t s' m k:
+        Star (L1 se) s t s' ->
+        star (fun _ => tensor_step) tt (tensor_st1 s m k) t (tensor_st1 s' m k).
+      Proof.
+        induction 1; [eapply star_refl | eapply star_step]; eauto.
+        constructor; auto.
+      Qed.
+
+      Lemma star_tensor_step2 s t s' m k:
+        Star (L2 se) s t s' ->
+        star (fun _ => tensor_step) tt (tensor_st2 s m k) t (tensor_st2 s' m k).
+      Proof.
+        induction 1; [eapply star_refl | eapply star_step]; eauto.
+        constructor; auto.
+      Qed.
+
+      Lemma plus_tensor_step1 s t s' m k:
+        Plus (L1 se) s t s' ->
+        plus (fun _ => tensor_step) tt (tensor_st1 s m k) t (tensor_st1 s' m k).
+      Proof.
+        destruct 1; econstructor; eauto using tensor_step1, star_tensor_step1.
+      Qed.
+
+      Lemma plus_tensor_step2 s t s' m k:
+        Plus (L2 se) s t s' ->
+        plus (fun _ => tensor_step) tt (tensor_st2 s m k) t (tensor_st2 s' m k).
+      Proof.
+        destruct 1; econstructor; eauto using tensor_step2, star_tensor_step2.
+      Qed.
 
     End WITH_SE.
 
-    Program Definition tensor_semantics' sk: semantics li_null (li@Ki) :=
+    Program Definition tensor_semantics' sk: semantics li_null (li_c@(K1 * K2)) :=
       {|
       activate se :=
         {|
@@ -129,8 +215,337 @@ Module Tensor.
           globalenv := tt;
         |};
       skel := sk;
-      footprint id := exists i, footprint (L i) id;
+      footprint id := footprint L1 id \/ footprint L2 id;
       |}.
 
   End COMP.
-End Tensor.
+
+  Section FSIM.
+
+    Context `(L1a: semantics li_null (li_c@K1a))
+            `(L1b: semantics li_null (li_c@K1b))
+            `(L2a: semantics li_null (li_c@K2a))
+            `(L2b: semantics li_null (li_c@K2b))
+            (cca: callconv (li_c@K1a) (li_c@K2a))
+            (ccb: callconv (li_c@K1b) (li_c@K2b))
+            (HL1: fsim_components cc_id cca L1a L2a)
+            (HL2: fsim_components cc_id ccb L1b L2b).
+    Context (INV: CallConv_Invariants cca ccb).
+    Context (se1 se2: Genv.symtbl) (w: ccworld (kcc_tensor cca ccb))
+            (Hse: match_senv (kcc_tensor cca ccb) w se1 se2)
+            (Hse1: Genv.valid_for (skel L1a) se1)
+            (Hse2: Genv.valid_for (skel L1b) se1).
+    Variable (sk: AST.program unit unit).
+
+    Inductive index: Type :=
+    | index1 (i: fsim_index HL1)
+    | index2 (i: fsim_index HL2).
+
+    Variant order: index -> index -> Prop :=
+    | order1 i1 i2: fsim_order HL1 i1 i2 -> order (index1 i1) (index1 i2)
+    | order2 i1 i2: fsim_order HL2 i1 i2 -> order (index2 i1) (index2 i2).
+
+    Arguments tensor_st1 {K1 K2 L1 L2}.
+    Arguments tensor_st2 {K1 K2 L1 L2}.
+    Variant match_states: index -> tensor_state L1a L1b
+                          -> tensor_state L2a L2b -> Prop :=
+    | match_states1 i s1 s2 m1 m2 k1 k2:
+        fsim_match_states HL1 se1 se2 (fst w) i s1 s2 ->
+        inv2 (snd w) (m1, k1) (m2, k2) ->
+        match_states (index1 i) (tensor_st1 s1 m1 k1)
+                     (tensor_st1 s2 m2 k2)
+    | match_states2 i s1 s2 m1 m2 k1 k2:
+        fsim_match_states HL2 se1 se2 (snd w) i s1 s2 ->
+        inv1 (fst w) (m1, k1) (m2, k2) ->
+        match_states (index2 i) (tensor_st2 s1 m1 k1)
+                     (tensor_st2 s2 m2 k2).
+
+    Local Lemma semantics_simulation sk1 sk2:
+      fsim_properties cc_id (kcc_tensor cca ccb) se1 se2 w
+                      (tensor_semantics' L1a L1b INV sk1 se1)
+                      (tensor_semantics' L2a L2b INV sk2 se2)
+                      index order match_states.
+    Proof.
+      constructor.
+      - intros [q1 [k1a k1b]] [q2 [k2a k2b]] s1 Hq H. inv H;
+        destruct ms as [m1a m1b] eqn: Hm1; destruct w as [wa wb] eqn: Hw;
+        destruct q2 as [? ? ? m2]; destruct (split m2) as [m2a m2b] eqn: Hm2.
+        + pose proof (fsim_lts HL1 _ _ (proj1 Hse) Hse1).
+          edestruct @fsim_match_initial_states as (idx & s' & H' & Hs); eauto.
+          instantiate (1 := ({| cq_vf := cq_vf; cq_sg := cq_sg; cq_args := cq_args; cq_mem := fst (m2a, m2b) |}, k2a)).
+          exploit match_query_core1. apply (proj1 Hq).
+          cbn in *. subst ms. rewrite Hm1. rewrite Hm2. auto.
+          eexists (index1 idx), (tensor_st1 s' (snd (split m2)) k2b).
+          split.
+          * constructor. congruence.
+          * constructor. subst w. apply Hs.
+            pose proof (inv2_pre _ _ _ _ _ (proj2 Hq)). cbn in H0.
+            cbn in *. subst ms. rewrite Hm1 in H0. rewrite Hm2 in H0. rewrite Hm2. subst w. apply H0.
+        + pose proof (fsim_lts HL2 _ _ (proj2 Hse) Hse2).
+          edestruct @fsim_match_initial_states as (idx & s' & H' & Hs); eauto.
+          instantiate (1 := ({| cq_vf := cq_vf; cq_sg := cq_sg; cq_args := cq_args; cq_mem := snd (m2a, m2b) |}, k2b)).
+          exploit match_query_core2. apply (proj2 Hq).
+          cbn in *. subst ms. rewrite Hm1. rewrite Hm2. auto.
+          eexists (index2 idx), (tensor_st2 s' (fst (split m2)) k2a).
+          split.
+          * constructor. congruence.
+          * constructor. subst w. apply Hs.
+            pose proof (inv1_pre _ _ _ _ _ (proj1 Hq)). cbn in H0.
+            cbn in *. subst ms; rewrite Hm1 in H0. rewrite Hm2 in H0. rewrite Hm2. subst w. apply H0.
+      - intros i s1 s2 [r1 [k1a k1b]] Hs H. inv H;
+        destruct w as [wa wb] eqn: Hw; inv Hs; cbn [fst snd] in *.
+        + pose proof (fsim_lts HL1 _ _ (proj1 Hse) Hse1).
+          edestruct @fsim_match_final_states as (r2 & H' & Hr); eauto. destruct r2 as [r2 k2a].
+          destruct r2 as [? m4] eqn: Hr2.
+          eexists (({|cr_retval := cr_retval; cr_mem := combine (m4, m3)|}, (k2a, k2))).
+          split.
+          * constructor. auto.
+          * constructor.
+            exploit match_reply_core1. apply Hr. eauto.
+            exploit inv2_post. apply H6. apply Hr. auto.
+        + pose proof (fsim_lts HL2 _ _ (proj2 Hse) Hse2).
+          edestruct @fsim_match_final_states as (r2 & H' & Hr); eauto. destruct r2 as [r2 k2b].
+          destruct r2 as [? m4] eqn: Hr2.
+          eexists (({|cr_retval := cr_retval; cr_mem := combine (m3, m4)|}, (k2, k2b))).
+          split.
+          * constructor. auto.
+          * constructor.
+            exploit inv1_post. apply H6. apply Hr. auto.
+            exploit match_reply_core2. apply Hr. eauto.
+      - intros. easy.
+      - intros. inv H; inv H0; destruct w as [wa wb] eqn: Hw.
+        + pose proof (fsim_lts HL1 _ _ (proj1 Hse) Hse1).
+          edestruct @fsim_simulation as (idx' & s2' & Hs2' & Hs'); eauto.
+          eexists (index1 idx'), (tensor_st1 s2' m2 k2).
+          split.
+          * destruct Hs2'; [left | right].
+            now apply plus_tensor_step1.
+            split; [apply star_tensor_step1 | constructor ]; apply H0.
+          * constructor; subst w. apply Hs'. auto.
+        + pose proof (fsim_lts HL2 _ _ (proj2 Hse) Hse2).
+          edestruct @fsim_simulation as (idx' & s2' & Hs2' & Hs'); eauto.
+          eexists (index2 idx'), (tensor_st2 s2' m2 k2).
+          split.
+          * destruct Hs2'; [left | right].
+            now apply plus_tensor_step2.
+            split; [apply star_tensor_step2 | constructor ]; apply H0.
+          * constructor; subst w. apply Hs'. auto.
+    Qed.
+  End FSIM.
+
+  Lemma tensor_compose_simulation'
+        `(cca: callconv (li_c@K1a) (li_c@K2a))
+        `(ccb: callconv (li_c@K1b) (li_c@K2b))
+        (INV: CallConv_Invariants cca ccb)
+        L1a L2a L1b L2b sk:
+    forward_simulation cc_id cca L1a L2a ->
+    forward_simulation cc_id ccb L1b L2b ->
+    linkorder (skel L1a) sk ->
+    linkorder (skel L1b) sk ->
+    forward_simulation cc_id (kcc_tensor cca ccb)
+                       (tensor_semantics' L1a L1b INV sk)
+                       (tensor_semantics' L2a L2b INV sk).
+  Proof.
+    intros [HL1] [HL2] Hk1 Hk2. constructor.
+    eapply Forward_simulation
+      with (order _ _ _ _ cca ccb HL1 HL2)
+           (match_states _ _ _ _ cca ccb HL1 HL2 INV).
+    - auto.
+    - intros. cbn.
+      rewrite (fsim_footprint HL1).
+      rewrite (fsim_footprint HL2). reflexivity.
+    - intros. eapply semantics_simulation; eauto.
+      eapply Genv.valid_for_linkorder; eauto.
+      eapply Genv.valid_for_linkorder; eauto.
+    - clear - HL1 HL2. intros [|].
+      + induction (fsim_order_wf HL1 i) as [x Hx IHx].
+        constructor. intros z Hxz. inv Hxz. apply IHx; eauto.
+      + induction (fsim_order_wf HL2 i) as [x Hx IHx].
+        constructor. intros z Hxz. inv Hxz. apply IHx; eauto.
+  Qed.
+
+End Layer.
+
+(* The code below doesn't work because it tries to define the tensor product
+   composition on transition systems with abstract data in general. It doesn't
+   work because we want to look into the queries and replies to obtain the
+   memory state, so to speak. Therefore, we turned to the concrete language
+   interface li_c. But it's still a problem that for transition systems L in
+   general we can't obtain the memory state from the (state L) *)
+
+(* Module Legacy. *)
+(*   (* Note for L@K: liA@K ↠ liB@K, the abstract state is only updated via external *)
+(*    calls. But for a transition system of type liA@K ↠ liB@K or even liA@K1 ↠ *)
+(*    liB@K2 in general, the abstract state may change at any transition step. But *)
+(*    here we limit our scope to the special case where internal steps do not *)
+(*    modify the abstract state *) *)
+
+(*   Section COMP. *)
+(*     (* TODO: notation precedence *) *)
+(*     Context {I} {K: I -> Type} *)
+(*             {liA liB} (L: forall i, semantics (liA@(K i)) (liB@(K i))). *)
+
+(*     (* Isomorphic to K0 * K1 * K2 * ... if indexed by natural number *) *)
+(*     Notation Ki := (forall i, K i). *)
+
+(*     Hypothesis I_dec: forall (i j: I), {i = j} + {i <> j}. *)
+
+(*     Definition update_at (k: Ki) (j: I) (kj: K j): Ki. *)
+(*     Proof. *)
+(*       intros i. destruct (I_dec i j). *)
+(*       - subst. exact kj. *)
+(*       - exact (k i). *)
+(*     Defined. *)
+
+(*     Section WITH_SE. *)
+(*       Context (se: Genv.symtbl). *)
+
+(*       (* Even though s has type (state (L i)), it should not be understood as the *)
+(*        state specific to the i-th component like in the flat composition. It *)
+(*        should be a directed join of all the states for the transition systems *)
+(*        being composed, where the state information from every component is *)
+(*        kept. It would be more appropriate that we define a new type for the *)
+(*        state that is independent of i, which is the way we deal with the *)
+(*        abstract data. *)
+
+(*        The all-inclusive abstract data k has a similar flavor but since two *)
+(*        abstract types K1 and K2 are not necessarily compatible they are first *)
+(*        lifted to K1*K2. Each field in the composite abstract data comes from its *)
+(*        respective component *) *)
+
+(*       (* An alternative approach would be to store  *) *)
+
+(*       (* (mem, k_i)  (k_1, k_2, ... k_n) *) *)
+(*       (* (m_1, m_2, m_3, .. m_n) *) *)
+
+(*       (* L_int ⊗ L_arr *) *)
+
+(*       (* L1 : 1 -> C ≤{1 -> cc1} L2 : 1 -> C@K2 *) *)
+(*       (* L3 : 1 -> C ≤{1 -> cc2} L4 : 1 -> C@K4 *) *)
+
+(*       (* cc1 : query(L1) ↔ query(L2) * K2 *) *)
+(*       (* cc2 : query(L3) ↔ qeury(L4) * K4 *) *)
+
+(*       (* L1 ⊗ L3 : 1 -> C *) *)
+(*       (* L2 ⊗ L4 : 1 -> C@(K2*K4) *) *)
+(*       (* L1 ⊗ L3 ≤{1 -> cc} L2 ⊗ L4 *) *)
+
+(*       (* cc : query(L1 ⊗ L3) ≅ mem ↔ query(L2 ⊗ L4) ≅ mem * K2 * K4 *) *)
+
+(*       Variant tensor_state := *)
+(*         tensor_st (i: I) (s: Smallstep_.state (L i)) (k: Ki). *)
+
+(*       Inductive tensor_step: tensor_state -> trace -> tensor_state -> Prop := *)
+(*       | step_intro i s t s' k: *)
+(*           Step (L i se) s t s' -> *)
+(*           tensor_step (tensor_st i s k) t (tensor_st i s' k). *)
+
+(*       Inductive tensor_initial_state: query (liB@Ki) -> tensor_state -> Prop := *)
+(*       | initial_state_intro i s k q: *)
+(*           initial_state (L i se) (q, k i) s -> *)
+(*           tensor_initial_state (q, k) (tensor_st i s k). *)
+
+(*       Inductive tensor_at_external: tensor_state -> query (liA@Ki) -> Prop := *)
+(*       | at_external_intro i s k q: *)
+(*           at_external (L i se) s (q, k i) -> *)
+(*           tensor_at_external (tensor_st i s k) (q, k). *)
+
+(*       (* This is the only transition where the abstract data is allowed to be *)
+(*        updated and only i-th state can be updated *) *)
+(*       Inductive tensor_after_external: *)
+(*         tensor_state -> reply (liA@Ki) -> tensor_state -> Prop := *)
+(*       | after_external_intro i s s' k k' r kr: *)
+(*           (forall j, i <> j -> k j = k' j) -> k' i = kr -> *)
+(*           after_external (L i se) s (r, kr) s' -> *)
+(*           tensor_after_external (tensor_st i s k) (r, k') (tensor_st i s' k'). *)
+
+(*       Inductive tensor_final_state: tensor_state -> reply (liB@Ki) -> Prop := *)
+(*       | final_state_intro i s k r: *)
+(*           final_state (L i se) s (r, k i) -> *)
+(*           tensor_final_state (tensor_st i s k) (r, k). *)
+
+(*       Lemma star_internal i s t s' k: *)
+(*         Star (L i se) s t s' -> *)
+(*         star (fun _ => tensor_step) tt (tensor_st i s k) t (tensor_st i s' k). *)
+(*       Proof. *)
+(*         induction 1; [eapply star_refl | eapply star_step]; eauto. *)
+(*         constructor; auto. *)
+(*       Qed. *)
+
+(*       Lemma plus_internal i s t s' k: *)
+(*         Plus (L i se) s t s' -> *)
+(*         plus (fun _ => tensor_step) tt (tensor_st i s k) t (tensor_st i s' k). *)
+(*       Proof. *)
+(*         destruct 1; econstructor; eauto using step_intro, star_internal. *)
+(*       Qed. *)
+
+(*     End WITH_SE. *)
+
+(*     Program Definition tensor_semantics' sk: semantics (liA@Ki) (liB@Ki) := *)
+(*       {| *)
+(*       activate se := *)
+(*         {| *)
+(*           step ge := tensor_step se; *)
+(*           initial_state := tensor_initial_state se; *)
+(*           at_external := tensor_at_external se; *)
+(*           after_external := tensor_after_external se; *)
+(*           final_state := tensor_final_state se; *)
+(*           globalenv := tt; *)
+(*         |}; *)
+(*       skel := sk; *)
+(*       footprint id := exists i, footprint (L i) id; *)
+(*       |}. *)
+
+(*   End COMP. *)
+
+(*   Require Import AbstractStateRel. *)
+(*   Require SmallstepLinking_. *)
+
+(*   Section FSIM. *)
+
+(*     Generalizable All Variables. *)
+
+(*     Context {I} (K1 K2: I -> Type) (Hi: Inhabited I) *)
+(*             `(L1: forall i, semantics (liA1@(K1 i)) (liB1@(K1 i))) *)
+(*             `(L2: forall i, semantics (liA2@(K2 i)) (liB2@(K2 i))) *)
+(*             (cca: forall i, callconv (liA1@(K1 i)) (liA2@(K2 i))) *)
+(*             (ccb: forall i, callconv (liB1@(K1 i)) (liB2@(K2 i))) *)
+(*             (HL: forall i, fsim_components (cca i) (ccb i) (L1 i) (L2 i)) *)
+(*             (se1 se2: Genv.symtbl) (w: ccworld (kcc_tensor ccb)) *)
+(*             (Hse: match_senv (kcc_tensor ccb) w se1 se2) *)
+(*             (Hse1: forall i, Genv.valid_for (skel (L1 i)) se1). *)
+(*     Variable (sk: AST.program unit unit). *)
+
+(*     Notation index := ({i & fsim_index (HL i)} * (forall i, K1 i) * (forall i, K2 i))%type. *)
+(*     Variant order: index -> index -> Prop := *)
+(*     | order_intro i x y kx1 kx2 ky1 ky2: *)
+(*         fsim_order (HL i) x y -> order (existT _ i x, kx1, kx2) (existT _ i y, ky1, ky2). *)
+
+(*     Variant match_states: index -> tensor_state L1 -> tensor_state L2 -> Prop := *)
+(*     | match_tensor_st i idx k1 k2 s1 s2 ks1 ks2: *)
+(*         fsim_match_states (HL i) se1 se2 (w i) idx s1 s2 -> *)
+(*         (forall j, j <> i -> ks1 j = k1 j /\ ks2 j = k2 j) -> *)
+(*         match_states (existT _ i idx, k1, k2) (tensor_st _ i s1 ks1) (tensor_st _ i s2 ks2). *)
+
+(*     Local Lemma semantics_simulation sk1 sk2: *)
+(*       fsim_properties (kcc_tensor cca) (kcc_tensor ccb) se1 se2 w *)
+(*                       (tensor_semantics' L1 sk1 se1) *)
+(*                       (tensor_semantics' L2 sk2 se2) *)
+(*                       index order match_states. *)
+(*     Proof. *)
+(*       split. *)
+(*       - intros [q1 kq1] [q2 kq2] s Hq H. inv H. *)
+(*         pose proof (fsim_lts (HL i) _ _ (Hse i) (Hse1 i)). *)
+(*         edestruct @fsim_match_initial_states as (idx & s' & Hs' & Hs); eauto. *)
+(*         eexists (existT _ i idx, kq1, kq2), _. split; econstructor; eauto. *)
+(*       - intros ((idx, k1), k2) s1 s2 [r kr] Hs H. inv H. *)
+(*         inv Hs. SmallstepLinking_.subst_dep. *)
+(*         pose proof (fsim_lts (HL i) _ _ (Hse i) (Hse1 i)). *)
+(*         edestruct @fsim_match_final_states as (r' & H' & Hr'); eauto. *)
+(*         destruct r' as [r' kr']. eexists (_, _). split. *)
+(*         + admit. *)
+(*         + intros j. *)
+(*     Abort All. *)
+
+(*   End FSIM. *)
+(* End Legacy. *)
